Adapt the proof of the invariant logic

src/prop/ReorderPromises.v
@@ -18,6 +18,7 @@ Require Import TView.
 Require Import Thread.
 Require Import Configuration.
 
+Require Import PFStep.
 Require Import PromiseConsistent.
 Require Import ReorderPromiseSame.
 
@@ -30,16 +31,23 @@ Inductive step_evt lang (e1 e2:Thread.t lang): Prop :=
     (STEP: Thread.step e e1 e2)
 .
 
-Inductive program_step_evt lang (e1 e2:Thread.t lang): Prop :=
-| program_step_evt_intro
+Inductive nonpf_step_evt lang (e1 e2:Thread.t lang): Prop :=
+| nonpf_step_evt_intro
     e
-    (STEP: Thread.program_step e e1 e2)
+    (STEP: nonpf_step e e1 e2)
 .
 
-Inductive promise_step_evt lang (e1 e2:Thread.t lang): Prop :=
-| promise_step_evt_intro
+Inductive pf_step_evt lang (e1 e2:Thread.t lang): Prop :=
+| pf_step_evt_intro
     e
-    (STEP: Thread.promise_step e e1 e2)
+    (STEP: pf_step e e1 e2)
+.
+
+Inductive tau_pf_step lang (e1 e2:Thread.t lang): Prop :=
+| tau_pf_step_intro
+    e
+    (STEP: pf_step e e1 e2)
+    (EVENT: ThreadEvent.get_event e = None)
 .
 
 Lemma step_evt_future lang (e1 e2:Thread.t lang)
@@ -76,8 +84,8 @@ Proof.
     splits; ss; etrans; eauto.
 Qed.
 
-Lemma promise_step_evt_future lang (e1 e2:Thread.t lang)
-      (STEP: promise_step_evt e1 e2)
+Lemma nonpf_step_evt_future lang (e1 e2:Thread.t lang)
+      (STEP: nonpf_step_evt e1 e2)
       (WF1: Local.wf e1.(Thread.local) e1.(Thread.memory))
       (SC1: Memory.closed_timemap e1.(Thread.sc) e1.(Thread.memory))
       (CLOSED1: Memory.closed e1.(Thread.memory)):
@@ -89,12 +97,13 @@ Lemma promise_step_evt_future lang (e1 e2:Thread.t lang)
   <<MEM_FUTURE: Memory.future e1.(Thread.memory) e2.(Thread.memory)>> /\
   <<STATE: e1.(Thread.state) = e2.(Thread.state)>>.
 Proof.
-  inv STEP. exploit Thread.promise_step_future; eauto. i. des.
-  inv STEP0. ss. esplits; eauto. refl.
+  inv STEP. inv STEP0. ss. guardH NONPF.
+  exploit Local.promise_step_future; eauto. i. des.
+  esplits; ss. refl.
 Qed.
 
-Lemma rtc_promise_step_evt_future lang (e1 e2:Thread.t lang)
-      (STEP: rtc (@promise_step_evt lang) e1 e2)
+Lemma rtc_nonpf_step_evt_future lang (e1 e2:Thread.t lang)
+      (STEP: rtc (@nonpf_step_evt lang) e1 e2)
       (WF1: Local.wf e1.(Thread.local) e1.(Thread.memory))
       (SC1: Memory.closed_timemap e1.(Thread.sc) e1.(Thread.memory))
       (CLOSED1: Memory.closed e1.(Thread.memory)):
@@ -108,13 +117,13 @@ Lemma rtc_promise_step_evt_future lang (e1 e2:Thread.t lang)
 Proof.
   revert WF1. induction STEP.
   - i. splits; ss; refl.
-  - i. exploit promise_step_evt_future; eauto. i. des.
+  - i. exploit nonpf_step_evt_future; eauto. i. des.
     exploit IHSTEP; eauto. i. des.
     splits; ss; etrans; eauto.
 Qed.
 
-Lemma tau_program_step_program_step_evt:
-  Thread.tau_program_step <3= program_step_evt.
+Lemma tau_pf_step_pf_step_evt:
+  tau_pf_step <3= pf_step_evt.
 Proof.
   i. inv PR. econs. eauto.
 Qed.
@@ -125,16 +134,30 @@ Proof.
   i. inv PR. econs. eauto.
 Qed.
 
-Lemma program_step_evt_step_evt:
-  program_step_evt <3= step_evt.
+Lemma pf_step_evt_step_evt:
+  pf_step_evt <3= step_evt.
 Proof.
-  i. inv PR. econs. eauto.
+  i. inv PR. inv STEP.
+  - econs. econs 1. econs. eauto.
+  - econs. econs 2. eauto.
 Qed.
 
-Lemma promise_step_evt_step_evt:
-  promise_step_evt <3= step_evt.
+Lemma tau_pf_step_tau_step:
+  tau_pf_step <3= Thread.tau_step.
 Proof.
-  i. inv PR. econs. eauto.
+  i. inv PR. inv STEP.
+  - econs.
+    + econs 1. econs. eauto.
+    + ss.
+  - econs.
+    + econs 2. eauto.
+    + ss.
+Qed.
+
+Lemma nonpf_step_evt_step_evt:
+  nonpf_step_evt <3= step_evt.
+Proof.
+  i. inv PR. inv STEP. econs. econs 1. econs. eauto.
 Qed.
 
 Lemma rtc_step_evt_promise_consistent
@@ -161,61 +184,67 @@ Lemma steps_pf_steps_aux
       (MEM1: Memory.closed e1.(Thread.memory)):
   exists n' e2,
     <<N: n' <= n>> /\
-    <<STEPS1: rtcn (@program_step_evt lang) n' e1 e2>> /\
-    <<STEPS2: rtc (@promise_step_evt lang) e2 e3>>.
+    <<STEPS1: rtcn (@pf_step_evt lang) n' e1 e2>> /\
+    <<STEPS2: rtc (@nonpf_step_evt lang) e2 e3>>.
 Proof.
   revert_until n. induction n using strong_induction; i.
   inv STEPS.
   { esplits; eauto. }
-  inv A12. inv STEP; cycle 1.
-  { exploit Thread.program_step_future; eauto. i. des.
+  inv A12. exploit pf_step_dec; eauto. i. des.
+  { exploit pf_step_future; eauto. i. des.
     exploit IH; eauto. i. des.
     esplits; cycle 1.
     + econs 2; eauto. econs; eauto.
     + auto.
     + omega.
   }
-  exploit Thread.promise_step_future; eauto. i. des.
+  exploit nonpf_step_future; eauto. i. des.
   exploit IH; try exact A23; try refl; eauto. i. des.
+  assert (CONS2: promise_consistent (Thread.local e2)).
+  { exploit rtcn_rtc; try exact A0; eauto. i.
+    exploit rtc_implies; (try by apply pf_step_evt_step_evt); eauto. i.
+    exploit rtc_step_evt_future; eauto. i. des.
+    eapply rtc_step_evt_promise_consistent; try exact CONS; eauto.
+    eapply rtc_implies; try exact STEPS2; eauto.
+    apply nonpf_step_evt_step_evt.
+  }
   inv STEPS1.
   { esplits; cycle 1.
     - eauto.
     - econs; eauto. econs. eauto.
     - omega.
   }
-  inversion A12. exploit Thread.program_step_future; eauto. i. des.
-  exploit reorder_promise_program; eauto.
+  inversion A12. exploit pf_step_future; eauto. i. des.
+  exploit reorder_nonpf_pf; eauto.
   { exploit rtcn_rtc; try exact A0; eauto. i.
     eapply rtc_step_evt_promise_consistent; try exact CONS; eauto.
     etrans.
-    - eapply rtc_implies; try exact x0; eauto.
-      apply program_step_evt_step_evt.
+    - eapply rtc_implies; try exact x1; eauto.
+      apply pf_step_evt_step_evt.
     - eapply rtc_implies; try exact STEPS2; eauto.
-      apply promise_step_evt_step_evt.
+      apply nonpf_step_evt_step_evt.
   }
   i. des.
-  exploit Thread.program_step_future; eauto. i. des.
-  unguardH STEP2. des.
-  - subst. esplits; cycle 1.
-    + econs 2; eauto. econs. eauto.
-    + auto.
-    + omega.
-  - exploit Thread.promise_step_future; try exact STEP2; eauto. i. des.
-    assert (STEPS: rtcn (step_evt (lang:=lang)) (S n) th1' e2).
+  - assert (STEPS: rtcn (step_evt (lang:=lang)) (S n) e1 e2).
     { econs 2.
-      - econs. econs 1. apply STEP2.
-      - eapply rtcn_imply; try exact A0. i. inv PR. econs; eauto.
+      - econs. eauto.
+      - eapply rtcn_imply; try exact A0. apply pf_step_evt_step_evt.
     }
-    exploit rtcn_rtc; eauto. i.
-    exploit rtc_step_evt_future; eauto. i. des.
     exploit IH; try exact STEPS; eauto.
     { omega. }
-    { eapply rtc_step_evt_promise_consistent; try exact CONS; eauto.
-      eapply rtc_implies; try exact STEPS2; eauto.
-      apply promise_step_evt_step_evt.
+    i. des. esplits; cycle 1; eauto.
+    + etrans; eauto.
+    + omega.
+  - assert (STEPS: rtcn (step_evt (lang:=lang)) (S n) th1' e2).
+    { econs 2.
+      - econs. econs 1. eauto.
+      - eapply rtcn_imply; try exact A0. apply pf_step_evt_step_evt.
     }
+    exploit pf_step_future; eauto. i. des.
+    exploit IH; try exact STEPS; eauto.
+    { omega. }
     i. des. esplits; cycle 1.
-    + econs; [|eauto]. econs; eauto.
+    + econs 2; eauto. econs. eauto.
     + etrans; eauto.
     + omega.
 Qed.
@@ -229,8 +258,8 @@ Lemma steps_pf_steps
       (SC1: Memory.closed_timemap e1.(Thread.sc) e1.(Thread.memory))
       (MEM1: Memory.closed e1.(Thread.memory)):
   exists e2,
-    <<STEPS1: rtc (@program_step_evt lang) e1 e2>> /\
-    <<STEPS2: rtc (@promise_step_evt lang) e2 e3>>.
+    <<STEPS1: rtc (@pf_step_evt lang) e1 e2>> /\
+    <<STEPS2: rtc (@nonpf_step_evt lang) e2 e3>>.
 Proof.
   apply rtc_rtcn in STEPS. des.
   exploit steps_pf_steps_aux; eauto. i. des.
@@ -247,61 +276,68 @@ Lemma tau_steps_pf_tau_steps_aux
       (MEM1: Memory.closed e1.(Thread.memory)):
   exists n' e2,
     <<N: n' <= n>> /\
-    <<STEPS1: rtcn (@Thread.tau_program_step lang) n' e1 e2>> /\
-    <<STEPS2: rtc (@promise_step_evt lang) e2 e3>>.
+    <<STEPS1: rtcn (@tau_pf_step lang) n' e1 e2>> /\
+    <<STEPS2: rtc (@nonpf_step_evt lang) e2 e3>>.
 Proof.
   revert_until n. induction n using strong_induction; i.
   inv STEPS.
   { esplits; eauto. }
-  inv A12. inv STEP; cycle 1.
-  { exploit Thread.program_step_future; eauto. i. des.
+  inv A12. exploit pf_step_dec; eauto. i. des.
+  { exploit pf_step_future; eauto. i. des.
     exploit IH; eauto. i. des.
     esplits; cycle 1.
     + econs 2; eauto. econs; eauto.
     + auto.
     + omega.
   }
-  exploit Thread.promise_step_future; eauto. i. des.
+  exploit nonpf_step_future; eauto. i. des.
   exploit IH; try exact A23; try refl; eauto. i. des.
+  assert (CONS2: promise_consistent (Thread.local e2)).
+  { exploit rtcn_rtc; try exact A0; eauto. i.
+    exploit rtc_implies; (try by apply tau_pf_step_pf_step_evt); eauto. i.
+    exploit rtc_implies; (try by apply pf_step_evt_step_evt); eauto. i.
+    exploit rtc_step_evt_future; eauto. i. des.
+    eapply rtc_step_evt_promise_consistent; try exact CONS; eauto.
+    eapply rtc_implies; try exact STEPS2; eauto.
+    apply nonpf_step_evt_step_evt.
+  }
   inv STEPS1.
   { esplits; cycle 1.
     - eauto.
     - econs; eauto. econs. eauto.
     - omega.
   }
-  inversion A12. exploit Thread.program_step_future; eauto. i. des.
-  exploit reorder_promise_program; eauto.
+  inversion A12. exploit pf_step_future; eauto. i. des.
+  exploit reorder_nonpf_pf; eauto.
   { exploit rtcn_rtc; try exact A0; eauto. i.
     eapply rtc_step_evt_promise_consistent; try exact CONS; eauto.
     etrans.
-    - eapply rtc_implies; try exact x0; eauto. i. inv PR.
-      eapply program_step_evt_step_evt. econs. eauto.
+    - eapply rtc_implies; try exact x1; eauto.
+      i. apply pf_step_evt_step_evt. apply tau_pf_step_pf_step_evt. ss.
     - eapply rtc_implies; try exact STEPS2; eauto.
-      apply promise_step_evt_step_evt.
+      apply nonpf_step_evt_step_evt.
   }
   i. des.
-  exploit Thread.program_step_future; eauto. i. des.
-  unguardH STEP2. des.
-  - subst. esplits; cycle 1.
-    + econs 2; eauto. econs; eauto.
-    + auto.
-    + omega.
-  - exploit Thread.promise_step_future; try exact STEP2; eauto. i. des.
-    assert (STEPS: rtcn (@Thread.tau_step lang) (S n) th1' e2).
+  - assert (STEPS: rtcn (Thread.tau_step (lang:=lang)) (S n) e1 e2).
     { econs 2.
-      - econs. econs 1. apply STEP2. inv STEP2. ss.
-      - eapply rtcn_imply; try exact A0. i. inv PR. econs; eauto.
+      - econs; eauto. etrans; eauto.
+      - eapply rtcn_imply; try exact A0. apply tau_pf_step_tau_step.
     }
-    exploit rtcn_rtc; eauto. i.
-    exploit Thread.rtc_step_future; eauto. i. des.
     exploit IH; try exact STEPS; eauto.
     { omega. }
-    { eapply rtc_step_evt_promise_consistent; try exact CONS; eauto.
-      eapply rtc_implies; try exact STEPS2; eauto.
-      apply promise_step_evt_step_evt.
+    i. des. esplits; cycle 1; eauto.
+    + etrans; eauto.
+    + omega.
+  - assert (STEPS: rtcn (Thread.tau_step (lang:=lang)) (S n) th1' e2).
+    { econs 2.
+      - econs. econs; eauto. by inv STEP2.
+      - eapply rtcn_imply; try exact A0. apply tau_pf_step_tau_step.
     }
+    exploit pf_step_future; eauto. i. des.
+    exploit IH; try exact STEPS; eauto.
+    { omega. }
     i. des. esplits; cycle 1.
-    + econs; [|eauto]. econs; eauto.
+    + econs 2; eauto. econs; eauto. etrans; eauto.
     + etrans; eauto.
     + omega.
 Qed.
@@ -315,17 +351,17 @@ Lemma tau_steps_pf_tau_steps
       (SC1: Memory.closed_timemap e1.(Thread.sc) e1.(Thread.memory))
       (MEM1: Memory.closed e1.(Thread.memory)):
   exists e2,
-    <<STEPS1: rtc (@Thread.tau_program_step lang) e1 e2>> /\
-    <<STEPS2: rtc (@promise_step_evt lang) e2 e3>>.
+    <<STEPS1: rtc (@tau_pf_step lang) e1 e2>> /\
+    <<STEPS2: rtc (@nonpf_step_evt lang) e2 e3>>.
 Proof.
   apply rtc_rtcn in STEPS. des.
   exploit tau_steps_pf_tau_steps_aux; eauto. i. des.
   exploit rtcn_rtc; eauto.
 Qed.
 
-Lemma promise_step_evt_bot
+Lemma nonpf_step_evt_bot
       lang e1 e2
-      (STEP: @promise_step_evt lang e1 e2)
+      (STEP: @nonpf_step_evt lang e1 e2)
       (PROMISE: e2.(Thread.local).(Local.promises) = Memory.bot):
   False.
 Proof.
@@ -341,12 +377,12 @@ Proof.
     rewrite Memory.bot_get. congr.
 Qed.
 
-Lemma rtc_promise_step_evt_bot
+Lemma rtc_nonpf_step_evt_bot
       lang e1 e2
-      (STEPS: rtc (@promise_step_evt lang) e1 e2)
+      (STEPS: rtc (@nonpf_step_evt lang) e1 e2)
       (PROMISE: e2.(Thread.local).(Local.promises) = Memory.bot):
   e1 = e2.
 Proof.
   exploit rtc_tail; eauto. i. des; ss.
-  exfalso. eapply promise_step_evt_bot; eauto.
+  exfalso. eapply nonpf_step_evt_bot; eauto.
 Qed.
